\input{BASE-HEAD}
\newcommand{\laClass}       {CS 210}
\newcommand{\laSemester}    {Spring 2018}
\newcommand{\laChapter}     {2.3}
\newcommand{\laType}        {Exercise}
\newcommand{\laPoints}      {5}
\newcommand{\laTitle}       {Mathematical Induction}
\newcommand{\laDate}        {}
\setcounter{chapter}{2}
\setcounter{section}{3}
\addtocounter{section}{-1}
\newcounter{question}

\toggletrue{answerkey}

\input{BASE-HEADER}

\input{INSTRUCTIONS-EXERCISE}

% ASSIGNMENT ------------------------------------ %

    \begin{enumerate}
        \item   
            \begin{itemize}
                \item[a.] $P(1) = $ {$1+1 = 2$, true}{}
                \item[b.] $P(3) = $ {$9+1 = 10$, false}{}
                \item[c.] $P(9) = $ {$81+1 = 81$, false}{}
            \end{itemize}

        \item
            \begin{itemize}
                \item[a.] $a_{1} = $    {1}{}
                \item[b.] $a_{2} = $    {$1 + 4 = 5$}{}
                \item[c.] $a_{3} = $    {$5 + 4 = 9$}{}
                \item[d.] $a_{m-1} = $  (Anywhere you see $k$, plug in $m-1$.)
                {$a_{m-2} + 4$}{}
            \end{itemize}

        \item
            \begin{itemize}
                \item[a.] $a_{1} = $    {$4 - 3 = 1$}{}
                \item[b.] $a_{3} = $    {$12 - 3 = 9$}{}
                \item[c.] $a_{5} = $    {$20 - 3 = 27$}{}
                \item[d.] $a_{m-1} = $  (Anywhere you see $n$, plug in $m-1$.) \\
                {$4(m-1) - 3 = 4m -4 -3 = 4m-7$}{}
            \end{itemize}

        \item
            \textbf{Step 1:}
            
            Recursive: $a_{1} = 5$; \tab
            Closed: $a_{1} = 2(1) + 3 = 5$
            \tab \checkmark
            
            \textbf{Step 2:}
            
            $a_{m} = 4 \cdot a_{m-1} + 2$

            \textbf{Step 3:}
            
            $ a_{m-1} = 2(m-1) + 3 \tab{}
            = 2m - 2 + 3 \tab{}
            = 2m + 1
            $

            \textbf{Step 4:}
            
            $ a_{m} = a_{m-1} + 2 $

            $ a_{m} = (2m+1) + 2 $

            $ a_{m} = 2m + 3 $

        \item
            \textbf{Step 1:}
            
            Recursive:
            $ a_{1} = 1 $
            \tab
            Closed:
            $ a_{1} = 2^{1} - 1  = 1$
            \tab \checkmark
            
            \textbf{Step 2:}
            
            $ a_{m} = 2 \cdot a_{m-1} + 1 $

            \textbf{Step 3:}
            
            $ a_{m-1} = 2^{m-1} - 1
            \tab{}
            = 2^{m} \cdot 2^{-1} - 1
            \tab{}
            = \frac{2^{m}}{2^{1}} - 1
            $

            \textbf{Step 4:}
            
            $ a_{m} = 2 \cdot a_{m-1} + 1 $
            
            $ a_{m} = 2^{1}(\frac{2^{m}}{2^{1}} - 1) + 1 $

            $ a_{m} = 2^{m} - 2 + 1 $

            $ a_{m} = 2^{m} - 1 $

        \item
            \textbf{Step 1:}
            
            Recursive: $b_{1} = 3$; \tab
            Closed: $b_{1} = 2^{2\cdot1} - 1 = 4 - 1 = 3$ \tab \checkmark
            
            \textbf{Step 2:}
            
            $b_{m} = 4 \cdot b_{m-1} + 3$
            
            \textbf{Step 3:}
            
            $ b_{m-1} = 2^{2(m-1)} - 1
            \tab = 2^{2m} \cdot 2^{-2} - 1
            \tab = \frac{ 2^{2m} }{2^{2}} - 1;$
            
            \textbf{Step 4:}
            
            $b_{m} = 4 a_{m-1} + 3$

            $b_{m} = 4 (\frac{2^{2m}}{2^{2}} - 1) + 3$

            $b_{m} = 2^{2}(\frac{2^{2m}}{2^{2}} - 1) + 3$

            $b_{m} = 2^{2m} - 4 + 3$

            $b_{m} = 2^{2m} - 1$

        \item
            \textbf{Step 1:}
            
                \begin{tabular}{l | p{4cm} | p{4cm} }
                    \textbf{ $i$ value } &
                    \textbf{ $ \sum_{i=1}^{n} (2i+4) $ } &
                    \textbf{ $n^{2} + 5n$ }
                    \\ \hline
                    $i = 1$ &
                        { $2(1)+4 = 6$ }{} &
                        { $1^{2} + 5(1) = 6$ }{} 

                    \\ 
                    $i = 2$ &
                        { $6 + 2(2)+4 = 14$ }{} &
                        { $2^{2} + 5(2) = 14$ }{} 

                    \\ 
                    $i = 3$ &
                        { $14 + 2(3) + 4 = 24$ }{} &
                        { $3^{2} + 5(3) = 9+15 = 24$ }{} 
                \end{tabular}
            
            \textbf{Step 2:}
            
                $ \sum_{i=1}^{m} (2i+4) = \sum_{i=1}^{m-1} (2i+4) + (2m+4)$

            \textbf{Step 3:}
            
                $ \sum_{i=1}^{m-1} (2i+4) = (m-1)^{2} + 5(m-1) $ ~\\
                $ \sum_{i=1}^{m-1} (2i+4) = m^{2} - 2m + 1 + 5m - 5 $ ~\\
                $ \sum_{i=1}^{m-1} (2i+4) = m^{2} + 3m - 4 $
                
            \textbf{Step 4:}
            
            $ \sum_{i=1}^{m} (2i+4) = (m^{2} + 3m - 4) + (2m+4) $ ~\\
            $ \sum_{i=1}^{m} (2i+4) = m^{2} + 5m $ ~\\
            This matches the original proposition.

        \item
            \textbf{Step 1:}
            
                \begin{tabular}{l | p{4cm} | p{4cm} }
                    \textbf{ $i$ value } &
                    \textbf{ $ \sum_{i=1}^{n} i $ } &
                    \textbf{ $ \frac{n(n+1)}{2} $ }
                    \\ \hline
                    $i = 1$ &
                        { $1$ }{} &
                        { $\frac{1(2)}{2} = 1$ }{} 

                    \\ 
                    $i = 2$ &
                        { $1 + 2 = 3$ }{} &
                        { $ \frac{2(2+1)}{2} = 3 $ }{} 

                    \\ 
                    $i = 3$ &
                        { $ 1 + 2 + 3 = 6$ }{} &
                        { $ \frac{3(3+1)}{2} = 6 $ }{} 
                \end{tabular}
            
            \textbf{Step 2:}
            
                $ \sum_{i=1}^{m} i = \sum_{i=1}^{m-1} (i) + m$

            \textbf{Step 3:}
            
                $ \sum_{i=1}^{m-1} i = \frac{(m-1)(m)}{2} $ ~\\
                $ \sum_{i=1}^{m-1} i = \frac{m^{2} - m}{2} $
                
            \textbf{Step 4:}
            
                $ \sum_{i=1}^{m} i = \frac{m^{2} - m}{2} + m $ ~\\
                $ \sum_{i=1}^{m} i = \frac{m^{2} - m}{2} + \frac{2m}{2} $ ~\\
                $ \sum_{i=1}^{m} i = \frac{m^{2} + m}{2} $ ~\\
                $ \sum_{i=1}^{m} i = \frac{m(m + 1)}{2} $ ~\\
                This matches the original proposition.
    \end{enumerate}
   
    
\input{BASE-FOOT}
